src/proof/store/deleteRange.v
@@ -30,6 +30,8 @@ From iris.algebra.lib Require Import dfrac_agree.
 From stdpp Require Import sorting.
 Local Open Scope Z_scope.
 From New.proof.store Require Import model value heap wp_private GetNode splitNode repair.
+From RecordUpdate Require Import RecordSet.
+Import RecordSetNotations.
 
 Section store_deleteRange.
 
@@ -103,8 +105,10 @@ Qed.
     the type's [len] field drops by the run's length, which is exactly what
     [num_visible] does under [flip_cell]. An already-tombstoned cell takes
     the [Indexable = false] branch, and the statement still holds on the nose
-    because [flip_cell] is the identity there. *)
-Lemma wp_store__deleteNode (s : loc) (types : gmap loc type_state)
+    because [flip_cell] is the identity there. Local: a stepping stone of
+    [wp_store__deleteRange], called while the range loop holds the pool apart
+    from the rest of the store. *)
+#[local] Lemma wp_store__deleteNode (s : loc) (types : gmap loc type_state)
     (p : loc) (ts : type_state) (k : nat) (c : item_cell) :
   types !! p = Some ts ->
   ty_cells ts !! k = Some c ->
@@ -214,33 +218,35 @@ Qed.
    the Go parameters are called [clock] and [length], but those are [YjsId]'s
    clock projection and [list]'s length in Rocq, and shadowing them breaks
    every [clock (item_id ...)] / [length (ic_run c)] below. *)
-Lemma wp_store__deleteRange (s : loc) (types : gmap loc type_state)
-    (client dclock dlen : w64) :
-  pool_invs types ->
-  {{{ is_pkg_init yjs ∗ own_store_items s types ∗ own_type_pool (DfracOwn 1) types }}}
+Lemma wp_store__deleteRange (s : loc) (st : store_state) (client dclock dlen : w64) :
+  {{{ is_pkg_init yjs ∗ own_store_cells s st }}}
     s @! (go.PointerType yjs.store) @! "deleteRange" #client #dclock #dlen
   {{{ (types' : gmap loc type_state) (covered : bool), RET #covered;
-      own_store_items s types' ∗ own_type_pool (DfracOwn 1) types' ∗
-      ⌜pool_invs types'⌝ ∗ ⌜delete_types_update_rel types types'⌝ ∗
+      own_store_cells s (st <| ss_types := types' |>) ∗
+      ⌜delete_types_update_rel (ss_types st) types'⌝ ∗
       ⌜range_no_overflow dclock dlen -> covered = true ->
          ids_tombstoned (range_ids client dclock dlen) (all_cells types')⌝ }}}.
 Proof using Type*.
-  move=> Hpool0.
-  iIntros (Φ) "(#Hpkg & Hitems & Htypes) HΦ".
+  iIntros (Φ) "(#Hpkg & Hcells) HΦ".
+  destruct st as [client0 k0 types bind pend pdel]. simpl.
+  iDestruct "Hcells" as "(Hfields0 & %Hinvs0)".
+  have Hpool0 : pool_invs types := proj1 Hinvs0.
+  have Hreg0 : registry_coh bind types := proj2 Hinvs0.
+  iAssert (own_store_cells s (MkStoreState client0 k0 types bind pend pdel)) with "[Hfields0]" as "Hcells".
+  { iFrame "Hfields0". iPureIntro. exact Hinvs0. }
   wp_method_call. wp_call. wp_call. wp_auto.
   iAssert (∃ (cur : w64) (cov : bool) (types_i : gmap loc type_state),
     "Hcur" ∷ cur_ptr ↦ cur ∗
     "Hcov" ∷ covered_ptr ↦ cov ∗
-    "Hitems" ∷ own_store_items s types_i ∗
-    "Htypes" ∷ (own_type_pool (DfracOwn 1) types_i) ∗
+    "Hcells" ∷ own_store_cells s (MkStoreState client0 k0 types_i bind pend pdel) ∗
     "%Hpool" ∷ ⌜pool_invs types_i⌝ ∗
     "%Hcurb" ∷ ⌜(uint.Z dclock <= uint.Z cur)%Z⌝ ∗
     "%Hcovj" ∷ ⌜range_no_overflow dclock dlen -> cov = true ->
         ids_tombstoned (range_ids client dclock (w64_word_instance.(word.sub) cur dclock))
                        (all_cells types_i)⌝ ∗
     "%Hfacts" ∷ ⌜delete_types_update_rel types types_i⌝)%I
-    with "[cur covered Hitems Htypes]" as "IH".
-  { iExists dclock, true, types. iFrame "cur covered Hitems Htypes". iPureIntro.
+    with "[cur covered Hcells]" as "IH".
+  { iExists dclock, true, types. iFrame "cur covered Hcells". iPureIntro.
     split_and!; [exact Hpool0 | lia | | exact (delete_types_update_rel_refl types)].
     (* nothing is covered yet: the span from [dclock] to [dclock] is empty *)
     move=> _ _ i Hi. exfalso. move: Hi.
@@ -250,8 +256,8 @@ Proof using Type*.
   wp_for "IH".
   wp_if_destruct; last first.
   { (* the range is exhausted: hand back the current pool *)
-    iApply ("HΦ" $! types_i cov). iFrame "Hitems Htypes". iPureIntro.
-    split_and!; [exact Hpool | exact Hfacts |].
+    iApply ("HΦ" $! types_i cov). simpl. iFrame "Hcells". iPureIntro.
+    split_and!; [exact Hfacts |].
     (* the loop stopped at [dclock + dlen], so its record covers the whole span *)
     move=> Hnw Hcov i Hi. apply (Hcovj Hnw Hcov i).
     move: Hi. rewrite !range_ids_elem.
@@ -260,15 +266,15 @@ Proof using Type*.
     move: n Hnw. rewrite /range_no_overflow /= => Hstop Hnw2. word. }
   wp_apply wp_NewId.
   have [Hfits [Hnodup [Hrangedisj Horiginclk]]] := Hpool.
-  wp_apply (wp_store__GetNode s _ types_i Hpool with "[$Hitems $Htypes]").
-  iIntros (nl found) "(Hitems & Htypes & %Hres)".
+  wp_apply (wp_store__GetNode s _ (MkStoreState client0 k0 types_i bind pend pdel) with "[$Hcells]").
+  iIntros (nl found) "(Hcells & %Hres)". simpl in Hres.
   wp_auto.
   destruct found; last first.
   { (* no node covers this char: skip it *)
     wp_auto. wp_for_post.
     iFrame "HΦ s client end".
     iExists (w64_word_instance.(word.add) cur (W64 1)), false, types_i.
-    iFrame "Hcur Hcov Hitems Htypes". iPureIntro.
+    iFrame "Hcur Hcov Hcells". iPureIntro.
     split_and!; [exact Hpool | word | by move=> _ | exact Hfacts]. }
   (* the covering cell, from the lookup *)
   destruct Hres as (cw & Hcwcov & Hcwloc).
@@ -276,9 +282,14 @@ Proof using Type*.
   have Hpool_i : pool_invs types_i by split_and!; assumption.
   wp_auto.
   wp_apply wp_NewId.
-  wp_apply (wp_store__splitAtAndGetRight s _ types_i cw Hcwcov Hpool
-              with "[$Hitems $Htypes]").
-  iIntros (rl types1) "(Hitems & Htypes & %Hpool1 & %Hstep1 & %HcR)".
+  wp_apply (wp_store__splitAtAndGetRight s _ (MkStoreState client0 k0 types_i bind pend pdel) cw Hcwcov
+              with "[$Hcells]").
+  iIntros (rl types1) "(Hcells & %Hstep1 & %HcR)".
+  iEval (simpl) in "Hcells".
+  iDestruct "Hcells" as "(Hfields1 & %Hinvs1)".
+  have Hpool1 : pool_invs types1 := proj1 Hinvs1.
+  have Hreg1 : registry_coh bind types1 := proj2 Hinvs1.
+  iDestruct "Hfields1" as "(Hclient & Hclock & HdeletedSet & Hitems & Hregistry & Htypes & Hpending & Hpdeletes)".
   iDestruct (own_type_pool_runs_wf with "Htypes") as %Hrunwf1.
   iDestruct (own_type_pool_id_bounds with "Htypes") as %Hbnds1.
   destruct HcR as (cR & HcRmem & HcRloc & HcRpar & HcRid).
@@ -342,9 +353,17 @@ Proof using Type*.
                 {| yjs.id.clientId' := cell_client cR;
                    yjs.id.clock' := w64_word_instance.(word.sub)
                      (w64_word_instance.(word.add) dclock dlen) (W64 1) |}
-                types1 cR HcRcovL Hpool1
-                with "[$Hitems $Htypes]").
-    iIntros (types2) "(Hitems & Htypes & %Hpool2 & %Hstep2 & %HcLs & %HcL)".
+                (MkStoreState client0 k0 types1 bind pend pdel) cR HcRcovL
+                with "[Hclient Hclock HdeletedSet Hitems Hregistry Htypes Hpending Hpdeletes]").
+    { iFrame "#".
+      iApply (own_store_cells_intro _ (MkStoreState client0 k0 types1 bind pend pdel) (conj Hpool1 Hreg1)
+                with "Hclient Hclock HdeletedSet Hitems Hregistry Htypes Hpending Hpdeletes"). }
+    iIntros (types2) "(Hcells & %Hstep2 & %HcLs & %HcL)".
+    iEval (simpl) in "Hcells".
+    iDestruct "Hcells" as "(Hfields2 & %Hinvs2)".
+    have Hpool2 : pool_invs types2 := proj1 Hinvs2.
+    have Hreg2 : registry_coh bind types2 := proj2 Hinvs2.
+    iDestruct "Hfields2" as "(Hclient & Hclock & HdeletedSet & Hitems & Hregistry & Htypes & Hpending & Hpdeletes)".
     iDestruct (own_type_pool_runs_wf with "Htypes") as %Hrunwf2.
     destruct HcL as (cL & HcLmem & HcLloc & HcLpar & HcLcln & HcLendn).
     destruct HcLs as (cL0 & HcL0mem & HcL0loc & _ & HcL0id).
@@ -375,7 +394,12 @@ Proof using Type*.
     wp_auto. wp_for_post.
     iFrame "HΦ s client end".
     iExists (w64_word_instance.(word.add) dclock dlen), cov, types3.
-    iFrame "Hcur Hcov Hitems Htypes".
+    have Hpool3 : pool_invs types3 := pool_invs_flip types2 pL tsL kL cL HpL HkL Hpool2.
+    have Hreg3 : registry_coh bind types3
+      := registry_coh_delete_step _ _ _ (delete_types_update_rel_of_flip types2 pL tsL kL cL HpL HkL) Hreg2.
+    iDestruct (own_store_cells_intro _ (MkStoreState client0 k0 types3 bind pend pdel) (conj Hpool3 Hreg3)
+                with "Hclient Hclock HdeletedSet Hitems Hregistry Htypes Hpending Hpdeletes") as "Hcells".
+    iFrame "Hcur Hcov Hcells".
     have Hdk3 : dead_chars_kept types_i types3.
     { eapply dead_chars_kept_trans;
         first exact (proj1 (proj2 (proj2 (proj2 (delete_types_update_rel_of_split _ _ _ Hstep1))))).
@@ -438,7 +462,12 @@ Proof using Type*.
     iFrame "HΦ s client end".
     iExists (w64_word_instance.(word.add) (ivR.(yjs.item.id').(yjs.id.clock'))
                (W64 (length (ivR.(yjs.item.content').(yjs.content.content'))))), cov, types3.
-    iFrame "Hcur Hcov Hitems Htypes".
+    have Hpool3 : pool_invs types3 := pool_invs_flip types1 pR tsR kR cR HpR HkR Hpool1.
+    have Hreg3 : registry_coh bind types3
+      := registry_coh_delete_step _ _ _ (delete_types_update_rel_of_flip types1 pR tsR kR cR HpR HkR) Hreg1.
+    iDestruct (own_store_cells_intro _ (MkStoreState client0 k0 types3 bind pend pdel) (conj Hpool3 Hreg3)
+                with "Hclient Hclock HdeletedSet Hitems Hregistry Htypes Hpending Hpdeletes") as "Hcells".
+    iFrame "Hcur Hcov Hcells".
     have Hdk3 : dead_chars_kept types_i types3.
     { eapply dead_chars_kept_trans;
         first exact (proj1 (proj2 (proj2 (proj2 (delete_types_update_rel_of_split _ _ _ Hstep1))))).
@@ -500,28 +529,30 @@ Qed.
     The buffer's own spans and the batch's are both consumed as VALUES (a
     span is a triple of machine words), so the batch comes back untouched
     and the new buffer is a fresh slice. *)
-Lemma wp_store__applyDeleteSpans (s : loc) (types : gmap loc type_state) (bind : gmap P loc)
-    (sp_sl : slice.t) (dq : dfrac) (pdel spans : list delete_span) :
-  {{{ is_pkg_init yjs ∗
-      own_store_core s types bind ∗ own_store_pending_deletes s pdel ∗
-      own_delete_spans sp_sl dq spans }}}
+Lemma wp_store__applyDeleteSpans (s : loc) (st : store_state)
+    (sp_sl : slice.t) (dq : dfrac) (spans : list delete_span) :
+  {{{ is_pkg_init yjs ∗ own_store_cells s st ∗ own_delete_spans sp_sl dq spans }}}
     s @! (go.PointerType yjs.store) @! "applyDeleteSpans" #sp_sl
   {{{ (types' : gmap loc type_state) (rest : list delete_span), RET #();
-      own_store_core s types' bind ∗ own_store_pending_deletes s rest ∗
+      own_store_cells s (st <| ss_types := types' |> <| ss_pending_deletes := rest |>) ∗
       own_delete_spans sp_sl dq spans ∗
-      ⌜delete_types_update_rel types types'⌝ ∗
+      ⌜delete_types_update_rel (ss_types st) types'⌝ ∗
       ⌜∃ D : gset YjsId,
          ids_tombstoned D (all_cells types') ∧
-         (∀ sp, sp ∈ pdel ++ spans -> delete_span_no_overflow sp ->
+         (∀ sp, sp ∈ ss_pending_deletes st ++ spans -> delete_span_no_overflow sp ->
             delete_span_ids sp ⊆ D ∪ delete_batch_ids rest)⌝ }}}.
 Proof using Type*.
-  iIntros (Φ) "(#Hpkg & Hcore & Hpdeletes & Hsp) HΦ".
-  iNamed "Hcore". iNamed "Hpdeletes".
-  have Hpool0 := Hpool.
+  iIntros (Φ) "(#Hpkg & Hcells & Hsp) HΦ".
+  destruct st as [client0 k0 types bind pend pdel]. simpl.
+  iDestruct "Hcells" as "(Hfields0 & %Hinvs0)".
+  have Hpool0 : pool_invs types := proj1 Hinvs0.
+  have Hreg : registry_coh bind types := proj2 Hinvs0.
+  iDestruct "Hfields0" as "(Hclient & Hclock & HdeletedSet & Hitems & Hregistry & Htypes & Hpending & Hpdeletes)".
+  iDestruct "Hpdeletes" as (pdel_sl) "(Hpddelf & Hpddel)".
   (* open the pure model: the decoded structs live only inside this proof *)
-  iNamed "Hpddel".
+  iDestruct "Hpddel" as (pdel_vs) "(Hspsl & Hspcap & %Hpdelmodel)".
   iDestruct "Hsp" as (spans_vs) "(Hspsl2 & Hspcap2 & %Hspansmodel)".
-  rename vs into pdel_vs. rename Hspmodel into Hpdelmodel.
+  simpl in Hpdelmodel.
   (* the pure lists ARE the denotations of the concrete ones; substituting
      them away keeps the rest of the proof over the structs the loop walks *)
   subst pdel spans.
@@ -555,35 +586,47 @@ Proof using Type*.
       "Hrest" ∷ rest_sl ↦* rest_vs ∗
       "Hrestcap" ∷ own_slice_cap yjs.deleteSpan.t rest_sl (DfracOwn 1) ∗
       "Hall" ∷ all_sl ↦* (pdel_vs ++ spans_vs) ∗
-      "Hitems" ∷ own_store_items s types_j ∗
-      "Htypes" ∷ (own_type_pool (DfracOwn 1) types_j) ∗
+      "Hcells" ∷ own_store_cells s (MkStoreState client0 k0 types_j bind pend []) ∗
       "%Hjb" ∷ ⌜(uint.nat j <= length (pdel_vs ++ spans_vs))%nat⌝ ∗
-      "%Hpoolj" ∷ ⌜pool_invs types_j⌝ ∗
       "%HdelDj" ∷ ⌜ids_tombstoned Dj (all_cells types_j)⌝ ∗
       "%HspanDj" ∷ ⌜∀ sp, sp ∈ take (uint.nat j) (pdel_vs ++ spans_vs) ->
           delete_span_no_overflow (delete_span_of_val sp) ->
           delete_span_ids (delete_span_of_val sp)
             ⊆ Dj ∪ delete_batch_ids (delete_span_of_val <$> rest_vs)⌝ ∗
       "%Hfactsj" ∷ ⌜delete_types_update_rel types types_j⌝)%I
-      with "[i rest Hrest Hrestcap Hall Hitems Htypes]" as "IH".
+      with "[i rest Hrest Hrestcap Hall Hclient Hclock HdeletedSet Hitems Hregistry Htypes Hpending Hpddelf]" as "IH".
     { iExists (W64 0), _, [], types, (∅ : gset YjsId).
-      iFrame "i rest Hrest Hrestcap Hall Hitems Htypes". iPureIntro.
-      split_and!; [word | exact Hpool0 | | | exact (delete_types_update_rel_refl types)].
+      iFrame "i rest Hrest Hrestcap Hall".
+      iSplitL.
+      { iApply (own_store_cells_intro _ (MkStoreState client0 k0 types bind pend []) Hinvs0
+                  with "Hclient Hclock HdeletedSet Hitems Hregistry Htypes Hpending [Hpddelf]").
+        iExists slice.nil. iFrame "Hpddelf". iExists [].
+        iSplitL; [iApply own_slice_nil | iSplitL; [iApply own_slice_cap_nil | done]]. }
+      iPureIntro.
+      split_and!; [word | | | exact (delete_types_update_rel_refl types)].
       - move=> i0 Hi0. exfalso. set_solver.
       - move=> sp0 Hsp0. exfalso. move: Hsp0.
         rewrite (_ : uint.nat (W64 0) = 0%nat); last word.
         rewrite take_0. apply elem_of_nil. }
     wp_for "IH".
     iDestruct (own_slice_len with "Hall") as %[Halllen _].
+    iDestruct "Hcells" as "(Hfieldsj & %Hinvsj)".
+    iDestruct "Hfieldsj" as "(Hclient & Hclock & HdeletedSet & Hitems & Hregistry & Htypes & Hpending & Hpdeletes)".
+    iDestruct "Hpdeletes" as (pd_sl) "(Hpddelf & Hpdnil)".
     wp_if_destruct; last first.
     { (* every span has been retried: install the leftover as the new buffer,
          and hand the whole thing back over the PURE model *)
       iApply ("HΦ" $! types_j (delete_span_of_val <$> rest_vs)).
-      iSplitL "Hitems Hregistry Htypes";
-        first (iApply (own_store_core_intro _ _ _ Hpoolj
-                         (registry_coh_delete_step _ _ _ Hfactsj Hreg) with "Hitems Hregistry Htypes")).
-      iSplitL "Hpddelf Hrest Hrestcap".
+      iAssert (own_store_pending_deletes s (delete_span_of_val <$> rest_vs))
+        with "[Hpddelf Hrest Hrestcap]" as "Hpdeletes".
       { iExists rest_sl. iFrame "Hpddelf". iExists rest_vs. by iFrame "Hrest Hrestcap". }
+      iSplitL "Hclient Hclock HdeletedSet Hitems Hregistry Htypes Hpending Hpdeletes".
+      { simpl.
+        have Hpoolj' : pool_invs types_j := proj1 Hinvsj.
+        have Hregj' : registry_coh bind types_j := proj2 Hinvsj.
+        iApply (own_store_cells_intro _ (MkStoreState client0 k0 types_j bind pend (delete_span_of_val <$> rest_vs))
+                  (conj Hpoolj' Hregj')
+                  with "Hclient Hclock HdeletedSet Hitems Hregistry Htypes Hpending Hpdeletes"). }
       iSplitL "Hspsl2 Hspcap2"; first (iExists spans_vs; by iFrame "Hspsl2 Hspcap2").
       iPureIntro. split_and!; [exact Hfactsj |].
       exists Dj. split; first exact HdelDj.
@@ -605,9 +648,14 @@ Proof using Type*.
     iDestruct ("Hgive" with "Hel") as "Hall".
     rewrite list_insert_id; last first.
     { replace (Z.to_nat (sint.Z j)) with (uint.nat j) by word. exact Hsp. }
-    wp_apply (wp_store__deleteRange s types_j _ _ _ Hpoolj
-                with "[$Hitems $Htypes]").
-    iIntros (types_j' cov) "(Hitems & Htypes & %Hpoolj' & %Hfactsj' & %Hcovj')".
+    wp_apply (wp_store__deleteRange s (MkStoreState client0 k0 types_j bind pend []) _ _ _
+                with "[Hclient Hclock HdeletedSet Hitems Hregistry Htypes Hpending Hpddelf Hpdnil]").
+    { iFrame "#".
+      iApply (own_store_cells_intro _ (MkStoreState client0 k0 types_j bind pend []) Hinvsj
+                with "Hclient Hclock HdeletedSet Hitems Hregistry Htypes Hpending [Hpddelf Hpdnil]").
+      iExists pd_sl. iFrame "Hpddelf Hpdnil". }
+    iIntros (types_j' cov) "(Hcells & %Hfactsj' & %Hcovj')".
+    iEval (simpl) in "Hcells".
     have Hfactsj'' : delete_types_update_rel types types_j'
       := delete_types_update_rel_trans _ _ _ Hfactsj Hfactsj'.
     (* the tombstone record of everything applied so far moves to the new pool *)
@@ -632,11 +680,11 @@ Proof using Type*.
     destruct cov.
     - (* the span landed in full: drop it, and record its ids *)
       wp_auto. wp_for_post.
-      iFrame "HΦ s Hpddelf Hspsl2 Hspcap2 Hallp Hallcap Hregistry".
+      iFrame "HΦ s Hspsl2 Hspcap2 Hallp Hallcap".
       iExists (w64_word_instance.(word.add) j (W64 1)), rest_sl, rest_vs, types_j',
         (Dj ∪ (if decide (delete_span_no_overflow (delete_span_of_val sp)) then delete_span_ids (delete_span_of_val sp) else ∅)).
-      iFrame "Hj Hrestp Hrest Hrestcap Hall Hitems Htypes".
-      iPureIntro. split_and!; [word | exact Hpoolj' | | | exact Hfactsj''].
+      iFrame "Hj Hrestp Hrest Hrestcap Hall Hcells".
+      iPureIntro. split_and!; [word | | | exact Hfactsj''].
       + move=> i0 /elem_of_union [Hi0 | Hi0]; first exact (Hmove Dj HdelDj i0 Hi0).
         destruct (decide (delete_span_no_overflow (delete_span_of_val sp))) as [Hnw | _]; last set_solver.
         exact (Hcovj' Hnw eq_refl i0 Hi0).
@@ -652,11 +700,11 @@ Proof using Type*.
       wp_apply (wp_slice_append with "[$Hrest $Hrestcap $Hssl]").
       iIntros (rest_sl') "(Hrest & Hrestcap & _)".
       wp_auto. wp_for_post.
-      iFrame "HΦ s Hpddelf Hspsl2 Hspcap2 Hallp Hallcap Hregistry".
+      iFrame "HΦ s Hspsl2 Hspcap2 Hallp Hallcap".
       iExists (w64_word_instance.(word.add) j (W64 1)), rest_sl', (rest_vs ++ [sp]), types_j',
         Dj.
-      iFrame "Hj Hrestp Hrest Hrestcap Hall Hitems Htypes".
-      iPureIntro. split_and!; [word | exact Hpoolj' | exact (Hmove Dj HdelDj) | | exact Hfactsj''].
+      iFrame "Hj Hrestp Hrest Hrestcap Hall Hcells".
+      iPureIntro. split_and!; [word | exact (Hmove Dj HdelDj) | | exact Hfactsj''].
       have Hgrow : delete_batch_ids (delete_span_of_val <$> rest_vs)
                  ⊆ delete_batch_ids (delete_span_of_val <$> (rest_vs ++ [sp])).
       { apply delete_batch_ids_mono => x Hx. rewrite fmap_app.
@@ -686,7 +734,7 @@ Proof using Type*.
   wp_apply (wp_slice_append with "[$Hall $Hallcap $Hsl0]").
   iIntros (all_sl') "(Hall & Hallcap & _)".
   wp_auto. wp_for_post.
-  iFrame "HΦ s spans Hitems Hregistry Htypes Hpddelf Hspcap2".
+  iFrame "HΦ s spans Hclient Hclock HdeletedSet Hitems Hregistry Htypes Hpending Hpddelf Hspcap2".
   iExists (w64_word_instance.(word.add) i (W64 1)), all_sl'.
   iFrame "Hi Hallp Hallcap Hspsl2".
   rewrite (_ : uint.nat (w64_word_instance.(word.add) i (W64 1))
@@ -726,11 +774,12 @@ Lemma wp_store__applyDeleteSpans_store (s_loc : loc) (γs : store_names)
   {{{ RET #(); own_store s_loc γs γh c h m pend ∗ own_delete_spans sp_sl dq spans }}}.
 Proof using Type*.
   iIntros (Φ) "(#Hpkg & Hstore & Hsp) HΦ".
-  iNamed "Hstore". iNamed "Hheap".
+  iNamed "Hstore".
   have [Hmtypes Hmdom] := Hregmodel.
-  wp_apply (wp_store__applyDeleteSpans s_loc types bind sp_sl dq pdel spans
-              with "[$Hcore $Hpdeletes $Hsp]").
-  iIntros (types' rest) "(Hcore & Hpdeletes & Hsp & %Hfacts & %_Hdels)".
+  wp_apply (wp_store__applyDeleteSpans s_loc (MkStoreState client k types bind pend pdel) sp_sl dq spans
+              with "[$Hcells $Hsp]").
+  iIntros (types' rest) "(Hcells & Hsp & %Hfacts & %_Hdels)".
+  iEval (simpl) in "Hcells". simpl in Hfacts.
   destruct Hfacts as (Harr & Hdom & Hlr & _ & Hcoord).
   (* the tombstone-set invariant follows the delete: both surgeries the loop
      performs (a split and a flip) only refine the live cells *)
@@ -761,11 +810,9 @@ Proof using Type*.
   { move=> parent ts' x Hts' Hx.
     destruct (Harr parent ts' Hts') as (ts & Hts & Heq).
     rewrite Heq in Hx. exact (Hctr parent ts x Hts Hx). }
-  iAssert (own_store_heap s_loc types' bind pend rest) with "[Hcore Hpending Hpdeletes]" as "Hheap".
-  { iFrame "Hcore Hpending Hpdeletes". }
   iApply "HΦ". iFrame "Hsp".
-  iExists client, k, deletedSetVal, rest, types', bind, acc.
-  iFrame "Hclient Hclock HdeletedSet Hheap Hseq HtypesAuth Hhist Hacc Hdelete_set".
+  iExists client, k, rest, types', bind, acc.
+  iFrame "Hcells Hseq HtypesAuth Hhist Hacc Hdelete_set".
   iFrame "Hclientpin Hpendcert Hbinds".
   iPureIntro. split_and!;
     [exact Hclientc | exact Hpendroot | exact Hpendbnd | exact Hregmodel' | exact Hhcoh
